Prove correctness of end-to-end compiler

compiler/proofs/pure_compilerProofScript.sml
@@ -7,18 +7,78 @@ open fixedPointTheory arithmeticTheory listTheory stringTheory alistTheory
      BasicProvers pred_setTheory relationTheory rich_listTheory finite_mapTheory;
 open pure_demandTheory
 open pure_cexpTheory pure_to_cakeProofTheory pureParseTheory
-     pure_inferenceProofTheory
+     pure_inferenceProofTheory state_to_cakeProofTheory
      pure_letrec_cexpProofTheory pure_demands_analysisProofTheory
-     fromSexpTheory simpleSexpParseTheory;
+     fromSexpTheory simpleSexpParseTheory pure_compilerTheory
+     pure_obs_sem_equalTheory;
 
 val _ = set_grammar_ancestry
           ["pure_cexp", "pure_to_cakeProof", "pureParse", "pure_inferenceProof",
-           "pure_letrec_cexpProof", "pure_demands_analysisProof", "fromSexp"];
+           "pure_letrec_cexpProof", "pure_demands_analysisProof", "fromSexp",
+           "simpleSexpParse", "state_to_cakeProof", "pure_compiler"];
 
 val _ = new_theory "pure_compilerProof";
 
+(* ---- misc ---- *)
 
+Definition string_to_ast_def:
+  string_to_ast s =
+    case parse_sexp (MAP (λx. (x,ARB)) s) of
+    | NONE => NONE
+    | SOME x => sexplist sexpdec x
+End
 
+Theorem string_to_ast_ast_to_string:
+  string_to_ast (ast_to_string p) = SOME p
+Proof
+  fs [string_to_ast_def,ast_to_string_def,AllCaseEqs()]
+  \\ fs [fromSexpTheory.sexplist_SOME,PULL_EXISTS]
+  \\ qabbrev_tac ‘l1 = print_sexp (listsexp (MAP decsexp p))’
+  \\ qabbrev_tac ‘l2 = MAP (λx. (x,ARB:locs)) l1’
+  \\ irule_at Any simpleSexpParseTheory.parse_print
+  \\ qexists_tac ‘MAP decsexp p’ \\ fs []
+  \\ fs [Abbr‘l2’] \\ fs [MAP_MAP_o,combinTheory.o_DEF,SF ETA_ss]
+  \\ irule fromSexpTheory.listsexp_valid
+  \\ fs [EVERY_MEM,MEM_MAP,PULL_EXISTS]
+QED
 
+(* ---- main theorem ---- *)
+
+Theorem pure_compiler_correct:
+  compile s = SOME t ⇒
+  ∃pure_ce ty cake_prog.
+    string_to_cexp s = SOME (pure_ce,ty) ∧
+    string_to_ast t = SOME cake_prog ∧
+    safe_exp (exp_of pure_ce) ∧
+    itree_rel
+       (itree_of (exp_of pure_ce))
+       (itree_semantics cake_prog)
+Proof
+  strip_tac \\ gvs [compile_def,AllCaseEqs()]
+  \\ fs [string_to_ast_ast_to_string]
+  \\ qabbrev_tac ‘e2 = demands_analysis (transform_cexp e1)’
+  \\ qsuff_tac ‘itree_of (exp_of e1) = itree_of (exp_of e2)’
+  >-
+   (disch_then $ rewrite_tac o single
+    \\ irule_at Any pure_to_cakeProofTheory.pure_to_cake_correct
+    \\ fs [cns_ok_def]
+    \\ imp_res_tac infer_types_SOME \\ fs [])
+  \\ qabbrev_tac ‘e3 = transform_cexp e1’
+  \\ qspec_then ‘e3’ mp_tac demands_analysis_soundness \\ fs []
+  \\ dxrule_then strip_assume_tac infer_types_SOME
+  \\ dxrule_then strip_assume_tac infer_types_SOME
+  \\ fs [] \\ strip_tac
+  \\ mp_tac safe_exp_app_bisim_F_IMP_same_itree
+  \\ gvs [pure_exp_relTheory.app_bisimilarity_eq]
+  \\ disch_then drule_all \\ fs []
+  \\ qspec_then ‘e1’ mp_tac transform_cexp_correct
+  \\ gvs [] \\ rpt strip_tac
+  \\ mp_tac bisimilarity_IMP_semantics_eq
+  \\ gvs [pure_exp_relTheory.app_bisimilarity_eq,GSYM pure_semanticsTheory.itree_of_def]
+  \\ disch_then drule \\ fs []
+  \\ disch_then irule
+  \\ unabbrev_all_tac
+  \\ imp_res_tac close_transform_cexp
+QED
 
 val _ = export_theory();
