typing/pure_typingScript.sml
@@ -223,6 +223,13 @@ Definition namespace_ok_def:
       MEM («Subscript»,[]) exndef
 End
 
+Overload append_ns = ``λns ns'. (FST ns ++ FST ns', SND ns ++ SND ns')``;
+
+Definition namespace_ok'_def:
+  namespace_ok' ns ⇔
+    namespace_ok ns ∧
+    ∃ns'. ns = append_ns initial_namespace ns'
+End
 
 (******************** Typing judgements ********************)
 
