compiler/backend/passes/proofs/pure_to_cakeProofScript.sml
@@ -59,8 +59,9 @@ QED
 Theorem pure_to_cake_correct:
   cexp_wf x ∧ closed (exp_of x) ∧ NestedCase_free x ∧
   safe_itree (itree_of (exp_of x)) ∧
-  state_to_cakeProof$state_namespace_ok ns ∧
-  state_to_cakeProof$cns_ok ns (IMAGE (IMAGE (explode ## I)) (pure_cexp$cns_arities x))
+  namespace_ok' ((I ## K ns) initial_namespace) ∧
+  state_to_cakeProof$cns_ok ((I ## K ns) initial_namespace)
+    (IMAGE (IMAGE (explode ## I)) (pure_cexp$cns_arities x))
   ⇒
   state_to_cakeProof$itree_rel
     (itree_of (exp_of x))
